Logic.lean
@@ -13,13 +13,30 @@ import Logic.Termination
 
 namespace multiSucc
 
-/--
-info: structure multiSucc.Kripke : Type
-number of parameters: 0
-fields:
-  multiSucc.Kripke.world : World
-  multiSucc.Kripke.branch : List Kripke
-constructor:
-  multiSucc.Kripke.mk (world : World) (branch : List Kripke) : Kripke
--/
-#guard_msgs in #print Kripke
+theorem Completeness (s : Sequent) (h : ∀ (m : Kripke), m.wf → s.evalR [] m ≠ TV.f) :
+    Nonempty (IG s) := by
+  contrapose! h
+  let res := automatedProof s.toSeq4 s.toSeq4.cap.card (by simp) (by simp [Sequent.toSeq4])
+  rcases res with ⟨(_ | ⟨p, ps⟩), h'⟩ | ⟨(_ | ⟨r, rs⟩), h'⟩
+  · contradiction
+  · have : s.toSeq4.toSeq = s := by
+      simp [Sequent.toSeq4, Sequent.Γ_getList, Sequent.Θ_getList, Sequent.Δ_getList]
+    rw [this] at p
+    absurd h
+    simp
+    use p
+  · contradiction
+  have := RIG.completeness _ r
+  simp_all
+  simp [Sequent.toSeq4, Sequent.Γ_getList, Sequent.Θ_getList, Sequent.Δ_getList] at this
+  obtain ⟨⟨h₁, h₃⟩, h₂⟩ := this
+  use r.getCM, r.cm_wf
+  grind
+
+theorem Completeness' (s : Sequent) (hp : IsEmpty (IG s)) :
+    ∃ (r : RIG s h), s.evalR h r.getCM = TV.f := by
+  sorry
+
+theorem Completeness (s : Sequent) (r : RIG s h) :
+    s.evalR h r.getCM = TV.f := by
+  sorry
