Logic/IG.lean
@@ -5,13 +5,13 @@ open multiSucc
 
 /-- `IG` is the inductive proof rules of Corsi and Tassi -/
 inductive IG : Sequent → Type
-  -- ∀ x Γ, x ++ Γ ⊢ x ++ Δ
+  /-- ∀ x Γ, x ++ Γ ⊢ x ++ Δ -/
   | ax :
     ∀ (x : Atom) (xs ys : List Form) (bl : List Imp),
       (hxs : .atom x ∈ xs) →
       (hys : .atom x ∈ ys) →
       IG ⟨↑xs, ↑bl, ↑ys⟩
-  -- ∀ Δ Γ, (⊥, Γ ⊢ Δ)
+  /-- ∀ Δ Γ, (⊥, Γ ⊢ Δ) -/
   | botl :
     ∀ (xs ys : List Form) (bl : List Imp),
       IG ⟨↑(⊥ :: xs), ↑bl, ↑ys⟩
@@ -19,44 +19,43 @@ inductive IG : Sequent → Type
     ∀ (xs ys : List Form) (bl : List Imp),
       IG ⟨↑xs, ↑bl, ↑ys⟩ →
       IG ⟨↑xs, ↑bl, ↑(⊥ :: ys)⟩
-  -- ∀ a b Γ Δ, (Γ, a, b ⊢ Δ) → (Γ, a ∧ b ⊢ Δ)
+  /-- ∀ a b Γ Δ, (Γ, a, b ⊢ Δ) → (Γ, a ∧ b ⊢ Δ) -/
   | andl :
     ∀ (a b : Form) (xs ys : List Form) (bl : List Imp),
       IG ⟨↑(a :: b :: xs), ↑bl, ↑ys⟩ →
       IG ⟨↑((a ∧∧ b) :: xs), ↑bl, ↑ys⟩
-  -- ∀ a b Γ Δ, (Γ ⊢ a, Δ) → (Γ ⊢ b, Δ) → (Γ ⊢ a ∧ b, Δ)
+  /-- ∀ a b Γ Δ, (Γ ⊢ a, Δ) → (Γ ⊢ b, Δ) → (Γ ⊢ a ∧ b, Δ) -/
   | andr :
     ∀ (a b : Form) (xs ys : List Form) (bl : List Imp),
       IG ⟨↑xs, ↑bl, ↑(a :: ys)⟩ →
       IG ⟨↑xs, ↑bl, ↑(b :: ys)⟩ →
       IG ⟨↑xs, ↑bl, ↑((a ∧∧ b) :: ys)⟩
-  -- ∀ a b Γ Δ, (a, Γ ⊢ Δ) → (b, Γ ⊢ Δ) → (a ∨ b, Γ ⊢ Δ)
+  /-- ∀ a b Γ Δ, (a, Γ ⊢ Δ) → (b, Γ ⊢ Δ) → (a ∨ b, Γ ⊢ Δ) -/
   | orl :
     ∀ (a b : Form) (xs ys : List Form) (bl : List Imp),
     IG ⟨↑(a :: xs), ↑bl, ↑ys⟩ →
     IG ⟨↑(b :: xs), ↑bl, ↑ys⟩ →
     IG ⟨↑((a ∨∨ b) :: xs), ↑bl, ↑ys⟩
-  -- ∀ a b Γ Δ , (Γ ⊢ a, b, Δ) → (Γ ⊢ a ∨ b, Δ)
+  /-- ∀ a b Γ Δ , (Γ ⊢ a, b, Δ) → (Γ ⊢ a ∨ b, Δ) -/
   | orr :
     ∀ (a b : Form) (xs ys : List Form) (bl : List Imp),
       IG ⟨↑xs, ↑bl, ↑(a :: b :: ys)⟩ →
       IG ⟨↑xs, ↑bl, ↑(( a ∨∨ b) :: ys)⟩
-  -- ∀ a b Γ Δ, (a, Γ ⊢ b) → ( Γ ⊢ a → b, Δ)
+  /-- ∀ a b Γ Δ, (a, Γ ⊢ b) → ( Γ ⊢ a → b, Δ) -/
   | impr :
     ∀ (a b : Form) (xs ys : List Form) (bl : List Imp),
       IG ⟨↑(a :: xs ++ bl.map Imp.toForm), {}, {b}⟩ →
       IG ⟨↑(xs), ↑bl, ↑((a ⊃ b) :: ys)⟩
-  -- ∀ a b Γ Δ, (a → b, Γ ⊢ a, Δ) → (b, Γ ⊢ Δ) → (a → b, Γ ⊢ Δ)
+  /-- ∀ a b Γ Δ, (a → b, Γ ⊢ a, Δ) → (b, Γ ⊢ Δ) → (a → b, Γ ⊢ Δ) -/
   | impl :
     ∀ (a b : Form) (xs ys : List Form) (bl : List Imp),
       IG ⟨↑xs, ↑(⟨a, b⟩ :: bl), ↑(a :: ys)⟩ →
       IG ⟨↑(b :: xs ), ↑bl, ↑ys⟩ →
       IG ⟨↑((a ⊃ b) :: xs), ↑bl, ↑ys⟩
-  -- ∀ a b Γ Δ, (Γ ⊢ b, Δ) → (Γ ⊢ a → b, Δ)
+  /-- ∀ a b Γ Δ, (Γ ⊢ b, Δ) → (Γ ⊢ a → b, Δ) -/
   | afort :
     ∀ (a b : Form) (xs ys : List Form) (bl : List Imp),
       IG ⟨↑xs, ↑bl, ↑(b :: ys)⟩ →
       IG ⟨↑xs, ↑bl, ↑((a ⊃ b) :: ys)⟩
 
 end multiSucc
-#min_imports
